Updated the documentation of the DNFP

Monad_Play Around/DNFP/Dutch_National_Flag_Monad_Definitions.thy
@@ -8,37 +8,40 @@ begin
 section\<open>Description of the DNFP-algortihm\<close>
 text\<open>The Dutch national flag problem is the problem of sorting an array into three different regions: A red-interval (0 in this version), A white-interval (1) and A Blue-interval (2)\<close>
 
+text\<open>The Dutch national flag problem is the problem of sorting an array into three different regions: A red-interval (0 in this version), A white-interval (1) and A Blue-interval (2)\<close>
+
 text\<open>The algorithm uses 3 variables to keep track of the three ranges:
 \begin{itemize}
-  \item Low: the red range is all indices before low
-  \item I: the index that is currently being checked, and the white range is between low up to I.
-  \item High: the blue range everything from high and up.
+  \item @{text Low}: the red range is all indexes before @{text low}
+  \item @{text I}: the index that is currently being checked, and the white range is between @{text low} up to @{text i}.
+  \item @{text High}: the blue range everything from @{text high} and up.
 \end{itemize}
 
-More information about the algortihm can be found: \url{https://en.wikipedia.org/wiki/Dutch_national_flag_problem}
+More information about the algorithm can be found: \url{https://en.wikipedia.org/wiki/Dutch_national_flag_problem}
 
 These three ranges have been used as invariants for the algorithm, and all definitions should preserve these.
 The relation between the variables has also been described as an invariant.
 
-The main proof of the program is to show the array is sorted in the final state. This can be shown given an array only containing {0,1,2}, and that initial satisfy the invariants should be sorted after the termination of the dnfp-function.
+The main proof of the program is to show the array is sorted in the final state. This can be shown given an array only containing the values of {0,1,2}. The array should also initially satisfy the invariants should be sorted after the termination of the dnfp-function.
 \<close>
 
 text\<open>The DNFP-algorithm has been split up in multiple definitions (non-recursive) based on the criteria that a definition should be as simple as possible. 
   A definition shouldn't contain more than a single conditional statement. 
-  The simplest definition has been used inside other definitions (see for example, the definition inc-lowbound that are used inside loop-update-action).
-Each of the definitions has been proved individually based on a pre-condition and post-condition. \<close>
+  The simplest definition has been used inside other definitions (see for example, the definition @{text inc_lowbound} that are used inside loop-update-action).
+Each of the definitions has been proved individually based on a pre-condition and post-condition.\<close>
 
-text\<open>The pre- and post-conditions are placed in a hierarchy where the conditions from the nested definitions inherit (and strength) the conditions from the outer definitions/functions.
-    This structure/hierarchy of the pre- a post-conditions makes it possible to use a lot of the already established lemmas of the simple definitions inside the compound definitions\<close>
+text\<open>The pre- and post-conditions are placed in a hierarchy where the conditions from the nested definitions inherit (and strengthen) the conditions from the outer definitions/functions.
+    This structure/hierarchy of the pre- a post-conditions makes it possible to use a lot of the already established lemmas of the simple definitions inside the compound definitions.
+    To benefit from this, it is essential to first do the proofs of the simple methods before proving the more complicated ones.\<close>
 
 text\<open>A thing to note about the use of the lemmas inside the compound methods is that can't be done if too much rewrite is done - because it makes it impossible for Isabelle to see the relationship between to post-conditions\<close>
 
-text\<open>Some of the pre- and post-conditions take more than one environment. This is because the post-condition contains some chceks about the relation between the variables in the initial and final state (for example the variable i is greater in the final state compared to the initial state).
-    In this case it is needed to capture the intial state (as an additional parameter of both the pre- and post-condition) inorder to use it in the post-condition\<close>
-
+text\<open>Some of the pre- and post-conditions take more than one environment as an argument. This is because the post-condition contains some checks about the relation between the variables in the initial and final state (for example, the variable @{text i} is greater in the final state compared to the initial state).
+    In this case, it is needed to capture the initial state (as an additional parameter of both the pre- and post-condition) to use it in the post-condition\<close>
 section\<open>Proof structure\<close>
 
-text\<open>The proofs are done using the rules defined in the State-Monad-HL. These rules are based on the book "" and are used to capture changes to the environment.\<close>
+text\<open>The proofs are done using the rules defined in the State-Monad-HL. These rules are based on the book 
+"Verification of Sequential and Concurrent Programs" and are used to capture changes to the environment.\<close>
 
 text\<open>The proof is built around rewriting an initial state into a final state. 
   The rewriting is done using the rules that capture the meaning of the program\<close>
@@ -46,19 +49,21 @@ text\<open>The proof is built around rewriting an initial state into a final sta
 text\<open>The proofs have all the same structure of a pre-condition that gets turned into a post-condition using the rewrite-rules.
     The strategy for doing this rewriting is, in most cases, as follows:
 \begin{enumerate}
-  \item Unfold the definitions in the lemma formula
+  \item Unfold the definitions in the lemma formula (pre- and post-conditions)
   \item Simp to extract the definition of the method
   \begin{itemize}
     \item Get is first - apply the get-rule. 
-    \item All quantifier is first  - apply the allI-rule to turn it into a LOOK HERE
+    \item All quantifier is first - apply the allI-rule to turn it into a LOOK HERE
     \item The final state is a conjunction - use the conj-rule-right to prove the goals separately 
     \item Put is first and gets followed by something - use the seq-rule to split it up. The seq rule shall contain what can be concluded from the put.
     \item Put followed by nothing (Usually the case after application of a  seq-rule) - use the simp to discharge the goal. If it doesn't prove the goal, use Sledgehammer, or rewrite the seq-rule.
   \end{itemize}
 \end{enumerate}
-\<close>
 
-  
+  The strategy above shall just be repeated until all sub-goals have been proven, and the proof is established. It seems very complicated, but it is, in fact, a very mechanical process.
+  In some of the compound methods, the already established lemmas can be used, which means a different strategy should be taken with a lot less rewriting.
+\<close>
+ 
 section\<open>Definitions of the monad environment\<close>
 type_synonym 'a array = "'a list"
 
@@ -69,6 +74,7 @@ record env =
   xs   :: "nat array"
 
 subsection\<open>Monad update functions\<close>
+text\<open>Each of the definitions takes an environment and a value of one of the variables. They update the value of the variable and outputs a new environment.\<close>
 definition high_Env:: "env \<Rightarrow> nat \<Rightarrow> env" where "high_Env s v = s \<lparr> high := v \<rparr>"
 definition low_Env:: "env \<Rightarrow> nat \<Rightarrow> env" where "low_Env s v = s \<lparr> low := v \<rparr>"
 definition i_Env:: "env \<Rightarrow> nat \<Rightarrow> env" where "i_Env s v = s \<lparr> i := v \<rparr>"
@@ -87,12 +93,14 @@ theorem put_i_rule: "spec (\<lambda>x. p () (x \<lparr> i := v \<rparr>)) (put i
 theorem put_xs_rule: "spec (\<lambda>x. p () (x \<lparr> xs := v \<rparr>)) (put xs_Env v) p"
   by (simp add: spec_def put_def get_state_def put_state_def xs_Env_def)
 
-section\<open>DNFP function definitions\<close>
+section\<open>Definitions of the methods inside DNFP\<close>
 text\<open>This section contains the basic definition of the dnfp-algorithm\<close>
 
 definition swap:: "'a array \<Rightarrow> nat \<Rightarrow> nat \<Rightarrow> 'a array" where
 "swap l x y \<equiv> (if x < length l \<and> y < length l then l[x := l!y, y := l!x] else l)"
 
+text\<open>The @{text inc_lowbound} method swaps elements at positions @{text i} and @{text low}. 
+    It afterwards increases both @{text i} and @{text low}\<close>
 definition inc_lowbound where
 "inc_lowbound \<equiv> do{
                   (l, s, j) \<leftarrow> get (\<lambda>e. (low e, xs e, i e));  
@@ -103,6 +111,8 @@ definition inc_lowbound where
                   put low_Env (Suc l)
                 }"
 
+text\<open>The @{text dec_highbound} method first decrements @{text high}. 
+    Secondly, it swaps elements at the new position @{text high} with the value at position @{text i}\<close>
 definition dec_highbound where
 "dec_highbound \<equiv> do{
                     h \<leftarrow> get high;
@@ -111,12 +121,14 @@ definition dec_highbound where
                     put xs_Env (swap s j h)
                 }"
 
+text\<open>The @{text inc_index} method increases the variable @{text i}.\<close>
 definition inc_index where
 "inc_index \<equiv> do{
                   j \<leftarrow> get i;
                   put i_Env (Suc j)
                 }"
 
+text\<open>The @{text loop_update_action} method performs a check of the value at position @{text i} and performs one of three actions.\<close>
 definition loop_update_action where
 "loop_update_action \<equiv> 
   do{
@@ -132,9 +144,9 @@ definition loop_update_action where
    }))
   }"
 
-section\<open>Invariants definitions\<close>
+section\<open>Definitions of the invariants\<close>
 text\<open>The invariants are taken from \url{https://en.wikipedia.org/wiki/Dutch_national_flag_problem} and more information about them can be seen in the general description of the algorithm.\<close>
-text\<open>It can be added that qunatifiers give the best proof-support of list/ranges compared to other list-functions.\<close>
+text\<open>An insight here is that quantifiers give the best proof-support of list/ranges compared to other list-functions.\<close>
 definition low_invariant_is_0_Env where
 "low_invariant_is_0_Env e \<equiv> (\<forall>x. x < (low e) \<longrightarrow> (xs e)!x = 0)"
 
@@ -152,18 +164,18 @@ definition dnfp_variables_invariants:: "env \<Rightarrow> bool" where
                       \<and> length (xs e) \<ge> high e
                       \<and> set (xs e) \<subseteq> {0,1,2}"
 
-text\<open>This post-condition states that the variables i, low and difference between high and i the  will never decrease.
-    High will never increase and the the multiset and length of the array will never change.\<close>
+text\<open>This post-condition states that the variables @{text i}, @{text low}, and the difference between @{text high} and @{text i} will never increase.
+    The variable @{text high} will never increase. And the multiset and length of the array will never be changed.\<close>
 definition dnfp_post where 
-"dnfp_post e e2 \<equiv> length (xs e) = length (xs e2)
-                  \<and> high e \<ge> high e2
-                  \<and> low e \<le> low e2
-                  \<and> i e \<le> i e2
-                  \<and> high e - i e \<ge> high e2 - i e2
-                  \<and> mset (xs e) = mset (xs e2)"
+"dnfp_post e e' \<equiv> length (xs e) = length (xs e')
+                  \<and> high e \<ge> high e'
+                  \<and> low e \<le> low e'
+                  \<and> i e \<le> i e'
+                  \<and> high e - i e \<ge> high e' - i e'
+                  \<and> mset (xs e) = mset (xs e')"
 
 subsection\<open>DNFP invariants\<close>
-text\<open>These definitions add the inviariant of the relationsship with the the different invariants on the range\<close>
+text\<open>These definitions add the invariant of the relationship with the different invariants on the ranges\<close>
 definition dnfp_inv1:: "env \<Rightarrow> bool" where 
 "dnfp_inv1  e \<equiv> dnfp_variables_invariants e
                 \<and> low_invariant_is_0_Env e"
@@ -179,8 +191,8 @@ definition dnfp_inv3:: "env \<Rightarrow> bool" where
 definition dnfp_inv :: "env \<Rightarrow> bool" where
 "dnfp_inv e \<equiv> ((dnfp_inv3 e) \<and> (dnfp_inv2 e) \<and> (dnfp_inv1 e))"
 
-subsubsection\<open>Other dnfp spec definitions\<close>
-text\<open>This is the final state of the algortihm\<close>
+subsubsection\<open>Other DNFP spec definitions\<close>
+text\<open>This is the final state of the algorithm. The main thing is that @{text i}, @{text high} is equal, and the invariants of the ranges\<close>
 definition dnfp_post_final_spec where
 "dnfp_post_final_spec e \<equiv> dnfp_inv e \<and> i e = high e"
 
@@ -197,6 +209,7 @@ definition i_high_equal::"nat \<Rightarrow> env \<Rightarrow> bool"  where
 definition dnfp_mon_spec_aux:: "nat \<Rightarrow> env \<Rightarrow> bool" where
 "dnfp_mon_spec_aux n e \<equiv> n = high e - i e \<and> dnfp_mon_spec e"
 
+text\<open>This is the main post-condition of the whole theory - the array gets sorted\<close>
 definition array_sorted where
 "array_sorted e \<equiv> sorted(xs e)"
 
@@ -207,7 +220,7 @@ text\<open>The post-condition is also for each of the definitions a little stron
 definition loop_update_action_pre:: "env \<Rightarrow> bool" where
 "loop_update_action_pre e \<equiv> dnfp_variables_invariants e \<and> high e > i e"
 
-text\<open>This is an example of a pre-condition that takes an extra env as a parameter. This is used to capture the initial state so it can be used in the post-condition.\<close>
+text\<open>This is an example of a pre-condition that takes an extra @{text env} as a parameter. This is used to capture the initial state so it can be used in the post-condition.\<close>
 definition loop_update_action_pre_aux:: "env \<Rightarrow> env \<Rightarrow> bool" where
 "loop_update_action_pre_aux e s \<equiv> s = e
                               \<and> loop_update_action_pre e"
@@ -230,8 +243,8 @@ definition loop_update_action_inv :: "env \<Rightarrow> bool" where
 "loop_update_action_inv s \<equiv> (dnfp_inv s \<and> loop_update_action_pre s)"
 
 section\<open>Definitions of the methods from inside the conditional-statement inside Loop update action\<close>
-text\<open>These definitions rely on the definitions on loop update action, but in the precondition they have an extra assumption that gets inferred from the conditions-statement inside loop-update-action\<close>
-text\<open>The post-condition is also for each of the definitions a little stronger compared to the more general loop_update-action-post\<close>
+text\<open>These definitions rely on the definitions on loop update action (@{text loop_update_action_pre}), but in the precondition they have an extra assumption that gets inferred from the conditions-statement inside loop-update-action\<close>
+text\<open>The post-condition does also make the post-condition a little stronger compared to the more general @{text loop_update_action_post}\<close>
 
 subsection\<open>Inc Lowbound definitions\<close>
 text\<open>This definitions is just the same as the ones for loop update action, but they are added with the information that can be infered from the conditional-statement. \<close>
