Monad_Play Around/DNFP/Dutch_National_Flag_Monad_Definitions_Lemmas.thy
@@ -5,7 +5,8 @@ begin
 
 section\<open>Aux. lemmas about values inside the array\<close>
 
-text\<open>These proofs have been made to make Isabelle able to inferer the correct value at position i in the array\<close>
+text\<open>These proofs have been made to make Isabelle able to infer the correct value at position @{text i} in the array.
+  The proof contains the same information in the assumptions that can be inferred from the conditional-statements and precondition.\<close>  
 lemma value_must_be_one : "\<lbrakk>xs e ! i e  \<noteq> 0 ; xs e! i e \<noteq> 2 ; i e < length (xs e) ; set(xs e) \<subseteq> {0,1,2}\<rbrakk> \<Longrightarrow> xs e ! i e = 1"
   by (smt insertE insert_subset mk_disjoint_insert nth_mem singletonD)
 
@@ -22,7 +23,7 @@ lemma value_must_be_one_aux : "\<lbrakk>\<not>xs e ! i e  > 1 ; \<not>xs e! i e 
   by linarith
 
 section\<open>Inc lowbound - proof\<close>
-text\<open>Inc lowbound will keep the relationship between variables and both the i and low variable will be increased\<close>
+text\<open>Inc lowbound will keep the relationship between variables and both the @{text i} and @{text low} variables will be increased\<close>
 lemma inc_lowbound_spec: "spec (inc_lowbound_pre e) inc_lowbound (GG (inc_lowbound_post e))"
   unfolding inc_lowbound_pre_def loop_update_action_pre_def dnfp_variables_invariants_def GG_def inc_lowbound_post_def loop_update_action_post_def dnfp_post_def
   apply(simp_all add: inc_lowbound_def)
@@ -118,7 +119,7 @@ lemma inc_lowbound_spec: "spec (inc_lowbound_pre e) inc_lowbound (GG (inc_lowbou
   by(simp add: spec_def put_def get_state_def put_state_def low_Env_def)
 
 subsection\<open>Invariants - inc lowbound\<close>
-text\<open>These proofs show that the invariants on the ranges are kept by a inc lowbound action\<close>
+text\<open>These proofs show that the invariants on the ranges are kept by a @{text inc_lowbound_action}\<close>
 lemma inc_lowbound_invariantRed: "spec inc_lowbound_inv1 inc_lowbound (GG dnfp_inv1)"
   unfolding inc_lowbound_inv1_def loop_update_action_pre_def  GG_def loop_update_action_inv1_def dnfp_inv1_def low_invariant_is_0_Env_def dnfp_variables_invariants_def
   apply(simp_all add: inc_lowbound_def)
@@ -267,7 +268,7 @@ lemma dec_highbound_spec: "spec (dec_highbound_pre e) dec_highbound (GG (dec_hig
   by (simp add: spec_def put_def put_state_def get_state_def xs_Env_def)
   
 subsection\<open>Invariants - dec highbound\<close>
-text\<open>These proofs show that the invariants on the ranges are kept by a dec highbound action\<close>
+text\<open>These proofs show that the invariants on the ranges are kept by a @{text dec_highbound_action}\<close>
 lemma dec_highbound_invariantRed: "spec dec_highbound_inv1 dec_highbound (GG dnfp_inv1)"
     unfolding dec_highbound_inv1_def dec_highbound_inv1_def loop_update_action_inv1_def dnfp_inv1_def dnfp_variables_invariants_def loop_update_action_pre_def GG_def low_invariant_is_0_Env_def
     apply(simp_all add: dec_highbound_def)
@@ -327,7 +328,8 @@ lemma inc_index_spec: "spec (inc_index_pre e) inc_index (GG (inc_index_post e))"
   by linarith
 
 subsection\<open>Invariants - inc index\<close>
-text\<open>These proofs show that the invariants on the ranges are kept by a inc index action. It can be noted that these proofs are very simple do the fact that the definition only contains one put-statement. 
+text\<open>These proofs show that the invariants on the ranges are kept by an @{text inc_index}-action. 
+  It can be noted that these proofs are straightforward since the definition only contains one put-statement. 
 And nothing follows the put-statement. It is therefore not necessary to introduce the seq-rule.)\<close>
 lemma inc_index_invariantRed: "spec inc_index_inv1 inc_index (GG dnfp_inv1)"
   unfolding inc_index_inv1_def loop_update_action_inv1_def dnfp_variables_invariants_def dnfp_inv1_def loop_update_action_pre_def  GG_def low_invariant_is_0_Env_def
@@ -518,14 +520,14 @@ lemma loop_update_action_invariantRed: "spec loop_update_action_inv1 loop_update
    apply (intro get_rule; intro allI; simp)
    by (simp add: spec_def get_def put_def get_state_def put_state_def i_Env_def)
 
- text\<open>The following proofs are mostly done using the already established lemmas of the definitions inside loop update action.\<close>
+text\<open>The following proofs are mostly done using the already established lemmas of the definitions inside loop update action. This can be seen from the lemmas used inside smt-statement\<close>
 lemma loop_update_action_invariantWhite: "spec loop_update_action_inv2 loop_update_action (GG dnfp_inv2)"
    unfolding loop_update_action_inv2_def GG_def
    apply(simp add: loop_update_action_def)
    apply (intro get_rule; intro allI; clarify)
    apply (intro cond_rule; simp)
    apply (smt GG_def case_prodD case_prodI2  inc_lowbound_inv2_def inc_lowbound_invariantWhite less_numeral_extra(1) loop_update_action_inv2_def spec_def)
-   apply (smt GG_def One_nat_def  dec_highbound_inv2_def dec_highbound_invariantWhite loop_update_action_inv2_def spec_def split_beta')
+   apply (smt GG_def One_nat_def dec_highbound_inv2_def dec_highbound_invariantWhite loop_update_action_inv2_def spec_def split_beta')
    by (smt GG_def One_nat_def Suc_less_eq inc_index_inv2_def inc_index_invariantWhite less_Suc_eq loop_update_action_inv2_def spec_def split_beta')
    
 lemma loop_update_action_invariantBlue: "spec loop_update_action_inv3 loop_update_action (GG dnfp_inv3)"
